code/experimental/P256/Hacl.Impl.ECDSA.P256SHA256.Signature.fst
@@ -1,0 +1,111 @@
+module Hacl.Impl.ECDSA.P256SHA256.Signature
+
+open FStar.HyperStack.All
+open FStar.HyperStack
+module ST = FStar.HyperStack.ST
+
+open Lib.IntTypes
+open Lib.Buffer
+
+open Hacl.Hash.SHA2
+open Hacl.Spec.P256.Definitions
+
+open Hacl.Spec.P256.Lemmas
+open Hacl.Spec.ECDSAP256.Definition
+open Hacl.Impl.LowLevel
+open Hacl.Spec.P256.Basic
+open Hacl.Spec.P256.Core
+
+open Hacl.Impl.ECDSA.MontgomeryMultiplication
+open Hacl.Impl.ECDSA.MM.Exponent
+open Hacl.Impl.P256.LowLevel
+open Hacl.Impl.LowLevel
+
+open Hacl.Spec.ECDSAP256.Definition
+
+open FStar.Mul
+
+(* yes, I know that it's a bad idea to include the full module, I will divide it at some point *)
+open Hacl.Impl.ECDSA.P256SHA256.Verification
+
+val ecdsa_signature_step01: mLen: size_t -> m: lbuffer uint8 mLen {uint_v mLen < pow2 61} -> hashAsFelem: felem -> 
+  Stack unit 
+    (requires fun h -> live h m /\ live h hashAsFelem)
+    (ensures fun h0 _ h1 -> True)
+
+let ecdsa_signature_step01 mLen m hashAsFelem  = 
+  push_frame(); 
+    let mHash = create (size 32) (u8 0) in  
+      let h0 = ST.get() in 
+    hash_256 m mLen mHash;
+      let h1 = ST.get() in 
+      assert(Seq.equal (as_seq h1 mHash) (Spec.Hash.hash Spec.Hash.Definitions.SHA2_256 (as_seq h0 m)));
+    toUint64 mHash hashAsFelem;
+    reduction_prime_2prime_order hashAsFelem hashAsFelem;
+  pop_frame()
+
+assume val l0: a: nat -> Lemma ((a * modp_inv2_prime (pow2 256) prime_p256_order) % prime_p256_order == fromDomain_ (a))
+
+val felem_add: arg1: felem -> arg2: felem ->  out: felem -> Stack unit 
+  (requires (fun h0 ->  
+    live h0 arg1 /\ live h0 arg2 /\ live h0 out /\ 
+    eq_or_disjoint arg1 out /\ eq_or_disjoint arg2 out /\
+    as_nat h0 arg1 < prime_p256_order /\ as_nat h0 arg2 < prime_p256_order
+   )
+  )
+  (ensures (fun h0 _ h1 -> modifies1 out h0 h1 /\ 
+      as_nat h1 out == (as_nat h0 arg1 + as_nat h0 arg2) % prime_p256_order 
+  ))
+
+
+let felem_add arg1 arg2 out = 
+  let h0 = ST.get() in   
+  let t = add4 arg1 arg2 out in 
+    reduction_prime_prime_2prime_with_carry2 t out out;
+  let h2 = ST.get() in 
+    admit()
+
+
+val ecdsa_signature_step6: kFelem: felem -> z: felem -> r: felem -> da: felem -> Stack unit
+  (requires fun h -> live h kFelem /\ live h z /\ live h r /\ live h da /\ as_nat h z < prime /\ as_nat h r < prime /\ as_nat h da < prime)
+  (ensures fun h0 _ h1 -> True)
+
+let ecdsa_signature_step6 kFelem z r da = 
+  push_frame();
+    let rda = create (size 4) (u64 0) in 
+    let zInv = create (size 4) (u64 0) in 
+	let h0 = ST.get() in 
+      montgomery_multiplication_ecdsa_module r da rda;
+	let h1 = ST.get() in 
+	assert(as_nat h1 rda = ((as_nat h0 r * as_nat h0 da) * modp_inv2_prime (pow2 256) prime_p256_order) % prime_p256_order);
+	assume (as_nat h0 r * as_nat h0 da > 0);
+	l0 (as_nat h0 r * as_nat h0 da);
+	assert(as_nat h1 rda = fromDomain_ (as_nat h0 r * as_nat h0 da));
+     fromDomainImpl z zInv;
+       let h2 = ST.get() in 
+       assert(as_nat h2 zInv = fromDomain_ (as_nat h0 z));
+     felem_add rda zInv zInv;  
+  pop_frame()
+
+
+val ecdsa_signature_core: mLen: size_t -> m: lbuffer uint8 mLen {uint_v mLen < pow2 61} ->  privKey: felem  -> k: felem -> result: point -> Stack unit
+  (requires fun h -> live h m )
+  (ensures fun h0 _ h1 -> True)
+
+
+let ecdsa_signature_core mLen m privKey k result = 
+  push_frame();
+    let hashAsFelem = create (size 4) (u64 0) in     
+    ecdsa_signature_step01 mLen m hashAsFelem;
+  pop_frame()
+
+val ecdsa_signature:  mLen: size_t -> m: lbuffer uint8 mLen {uint_v mLen < pow2 61} ->   privKey: felem -> k: felem -> result: point -> Stack bool
+  (requires fun h -> live h privKey /\ live h k /\ live h result /\ live h m)
+  (ensures fun h0 _ h1 -> True)
+
+let ecdsa_signature mLen m privKey k result = 
+  let f = isMoreThanZeroLessThanOrderMinusOne privKey in 
+  let s = isMoreThanZeroLessThanOrderMinusOne k in 
+
+  ecdsa_signature_core mLen m privKey k result; 
+  f && s
